Source/IntegrationTests/TestFiles/LitTests/LitTest/dafny0/CanCall.dfy
@@ -61,3 +61,36 @@ module ArraySeqInit {
   }
 
 }
+
+module QuantifierBeforeOtherConjunct {
+  datatype List<T> = Nil | Cons(head: T, tail: List)
+
+  function Length(list: List): nat {
+    match list
+    case Nil => 0
+    case Cons(_, tl) => 1 + Length(tl)
+  }
+
+  function Occurrences(x: int, list: List<int>): nat
+  {
+    match list
+    case Nil => 0
+    case Cons(y, tl) => (if x == y then 1 else 0) + Occurrences(x, tl)
+  }
+
+  function Partition(x: int, l: List<int>): (result: (List<int>, List<int>))
+    ensures
+      && (forall y :: Occurrences(y, result.0) == if y <= x then Occurrences(y, l) else 0)
+      && Length(l) == Length(result.0) + Length(result.1)
+
+  lemma CallPartition(x: int, l: List<int>) returns (aaa: List<int>, bbb: List<int>)
+    requires l.Cons? && l.head <= x
+    ensures
+      && (forall y :: Occurrences(y, aaa) == if y <= x then Occurrences(y, l) else 0)
+      && Length(l) == Length(aaa) + Length(bbb)
+  {
+    var (lo, hi) := Partition(x, l.tail);
+    aaa := Cons(l.head, lo);
+    bbb := hi;
+  }
+}
